verified nondet

fairness/lawyer/examples/nondet/nondet.v
@@ -79,16 +79,16 @@ Section Nondet.
   Context {OBLS_AMU__f: forall τ, @AMU_lift_MU__f _ _ _ τ oGS' _ EM _ ⊤}.
   Context {NO_OBS_POST: ∀ τ v, obls τ ∅ -∗ fork_post τ v}.
 
-  Definition nondet_LS_LB := 10. 
+  Definition nondet_LS_LB := 30. 
+  Hypothesis (LS_LB: nondet_LS_LB <= LIM_STEPS).
 
-  Lemma incr_loop_spec `{NondetG Σ} τ π cnt flag s__f
-    (LS_LB: nondet_LS_LB <= LIM_STEPS):
+  Lemma incr_loop_spec `{NondetG Σ} τ π cnt flag s__f:
     {{{ th_phase_eq τ π ∗ cp_mul π d0 10 ∗
         obls τ ∅ ∗ ep s__f π d0 ∗
         nondet_inv cnt flag s__f }}}
       incr_loop #cnt #flag @ τ
     {{{ v, RET v; obls τ ∅ }}}.
-  Proof using OBLS_AMU ODl LEl.
+  Proof using OBLS_AMU ODl LEl LS_LB.
     iIntros (Φ) "(PH & CPS & OB & #EP & #INV) POST".
     iLöb as "IH". 
     rewrite /incr_loop.
@@ -134,7 +134,7 @@ Section Nondet.
       
       MU_by_BOU.
       iMod (increase_eb_upd with "EB") as "#EB'".
-      { rewrite /nondet_LS_LB in LS_LB. lia. }
+      { unfold nondet_LS_LB in LS_LB. lia. }
       iModIntro. burn_cp_after_BOU.
       iApply wp_value.
 
@@ -165,10 +165,12 @@ Section Nondet.
 
   Lemma alloc_nondet_inv `{NondetPreG Σ} τ cnt flag:
     cnt ↦ #(0%nat) -∗ flag ↦ #false -∗ obls τ ∅ -∗
-    BOU ∅ 1 (∃ s__f (ND: NondetG Σ), nondet_inv cnt flag s__f ∗ obls τ {[ s__f ]}).
+    BOU ∅ 1 (∃ s__f (ND: NondetG Σ), nondet_inv cnt flag s__f ∗ 
+                                    obls τ {[ s__f ]} ∗ sgn s__f l__f None ∗ tok).
   Proof using.
     iIntros "CNT FLAG OB".
     iMod (OU_create_sig _ _ l__f with "[$]") as "(%s__f & SGN & OB & _)".
+    iDestruct (sgn_get_ex with "[$]") as "[SGN #SGN']".
     iMod (own_alloc (Excl tt: exclR unitO)) as (γ) "TOK".
     { done. }
 
@@ -180,10 +182,105 @@ Section Nondet.
     iIntros "EB".
 
     set (ND := {| γ__tok := γ |}).
-    iMod (inv_alloc nondet_ns _ (nondet_inv_inner _ _ _) with "[-OB]") as "#?".
+    iMod (inv_alloc nondet_ns _ (nondet_inv_inner _ _ _) with "[-OB TOK]") as "#?".
     { do 2 iExists _. iNext. iFrame. iLeft. by iFrame. }
 
     iModIntro. do 2 iExists _. rewrite union_empty_l_L. iFrame "#∗".
   Qed.
+
+  (* TODO: move *)
+  Lemma ep_weaken s π1 π2 d
+    (PH_LE: phase_le π1 π2):
+    ep s π1 d -∗ ep s π2 d.
+  Proof using.
+    rewrite /ep. iIntros "(%&?&%)".
+    iExists _. iFrame. iPureIntro. etrans; eauto.
+  Qed.     
+
+  Theorem nondet_spec `{NondetPreG Σ} τ π:
+    {{{ th_phase_eq τ π ∗ cp_mul π d1 2 ∗ obls τ ∅ }}}
+      nondet #() @ τ
+    {{{ vn, RET vn; ∃ (n: nat), ⌜ vn = #n ⌝ ∗ exc_lb n ∗ obls τ ∅ }}}.
+  Proof.
+    iIntros (Φ) "(PH & CPS1 & OB) POST". rewrite /nondet.
+
+    split_cps "CPS1" 1. rewrite -cp_mul_1.
+    pure_step_hl. MU_by_BOU.
+    iMod (first_BOU with "[$]") as "[CPS #EB]".
+    { apply DEG01. }
+    BOU_burn_cp.
+
+    wp_bind (ref _)%E.
+    iApply sswp_MU_wp; [done| ]. iApply wp_alloc. iIntros "!> %cnt CNT _".
+    MU_by_burn_cp. iApply wp_value.
+
+    wp_bind (Rec _ _ _)%E. pure_steps.
+
+    wp_bind (ref _)%E.
+    iApply sswp_MU_wp; [done| ]. iApply wp_alloc. iIntros "!> %flag FLAG _".
+    MU_by_BOU.
+    iApply (BOU_weaken ∅); [reflexivity| set_solver| ..].
+    { eauto. }
+    iMod (alloc_nondet_inv with "[$] [$] [$]") as "(%s__f & %ND & #INV & OB & #SGN0 & TOK)".
+    { unfold nondet_LS_LB in LS_LB. lia. }
+    iMod (create_ep_upd with "[$] [$] [$]") as "(#EP & _ & PH)".
+    { apply DEG01. }
+    { unfold nondet_LS_LB in LS_LB. lia. }
+    BOU_burn_cp. iApply wp_value.
+
+    wp_bind (Rec _ _ _)%E. pure_steps.
+
+    wp_bind (Fork _)%E.
+    iApply sswp_MUf_wp. iIntros (τ') "!>".
+    split_cps "CPS" 1.
+
+    MU__f_by_BOU (∅: gset SignalId). 
+    iModIntro. iSplitR "CPS' PH OB". 
+    2: { iExists _. rewrite cp_mul_1. by iFrame. }
+    iIntros "(%π1 & %π2 & PH1 & OB1 & PH2 & OB2 & [%PH_LT1 %PH_LT2])".
+
+    split_cps "CPS" 10. 
+    iSplitR "CPS PH1 OB1 POST TOK".
+    { erewrite ep_weaken; [| apply PH_LT2].
+      erewrite cp_mul_weaken; [| apply PH_LT2| reflexivity].
+      rewrite intersection_empty_r_L.
+      iApply (incr_loop_spec with "[-]").
+      { iFrame "#∗". }
+      iIntros "!> % OB". by iApply NO_OBS_POST. }
+
+    erewrite cp_mul_weaken; [| apply PH_LT1| reflexivity]. iRename "PH1" into "PH".
+    wp_bind (Rec _ _ _)%E. pure_steps.
+
+    wp_bind (_ <- _)%E.
+    iApply wp_atomic.
+    iInv "INV" as "inv" "CLOS". iModIntro.
+    rewrite {1}/nondet_inv_inner. iDestruct "inv" as ">(%c & %f & CNT & FLAG & CASES & EXc)".
+    iDestruct "CASES" as "[[-> SGN] | [-> TOK']]".
+    2: { iCombine "TOK TOK'" as "TOK". by iDestruct (own_valid with "TOK") as %V. }
+    iApply sswp_MU_wp; [done| ]. iApply (wp_store with "[$]"). iIntros "!> FLAG".
+    MU_by_BOU.
+    iMod (OU_set_sig with "[$] [$]") as "[SGN OB]".
+    { set_solver. }
+    { unfold nondet_LS_LB in LS_LB. lia. }
+    BOU_burn_cp. iApply wp_value.
+    iMod ("CLOS" with "[CNT FLAG TOK EXc]") as "_".
+    { do 2 iExists _. iFrame. iNext. iRight. by iFrame. }
+    iModIntro. 
+    
+    wp_bind (Rec _ _ _)%E. pure_steps.
+    wp_bind (! _)%E. 
+    clear c. 
+    iApply wp_atomic.
+    iInv "INV" as "inv" "CLOS". iModIntro.
+    rewrite {1}/nondet_inv_inner. iDestruct "inv" as ">(%c & %f & CNT & FLAG & CASES & #EXc)".
+    iApply sswp_MU_wp; [done| ]. iApply (wp_load with "CNT"). iIntros "!> CNT".
+    MU_by_burn_cp. iApply wp_value. 
+    iMod ("CLOS" with "[CNT FLAG CASES]") as "_".
+    { do 2 iExists _. iFrame "#∗". }
+    iModIntro.
+
+    iApply "POST". iExists _. iFrame "#∗". iSplit; [done| ].
+    iApply (obls_proper with "[$]"). set_solver.
+  Qed.    
   
 End Nondet.
